examples/map/MapMAproof.v
@@ -1,4 +1,4 @@
-Require Import HoareDef MapHeader MapM MapA SimModSem.
+(* Require Import HoareDef MapHeader MapM MapA SimModSem.
 Require Import Coqlib.
 Require Import ImpPrelude.
 Require Import Skeleton.
@@ -394,4 +394,4 @@ Section SIMMODSEM.
 
 
 End SIMMODSEM.
-
+ *)
