examples/tinytutorial/init/InitIAProof.v
@@ -1,0 +1,136 @@
+Require Import Coqlib.
+Require Import ImpPrelude.
+Require Import STS.
+Require Import Behavior.
+Require Import ModSem.
+Require Import Skeleton.
+Require Import PCM.
+Require Import HoareDef IPM.
+Require Import sProp sWorld World SRF.
+Require Import InitI InitA InitRA.
+Require Import Relation_Operators.
+Require Import RelationPairs.
+
+Require Import SimModSemFacts IProofMode IRed ITactics.
+
+
+Set Implicit Arguments.
+
+Section SIM.
+  Context `{_I: InitRA.t}.
+
+  Variable GlobalStb: Sk.t -> gname -> option fspec.
+
+  Let Ist : Any.t -> Any.t -> iProp := 
+    (fun st_src st_tgt => 
+          (pending ∗ (∃n:Z, ⌜st_src = n↑ /\ st_tgt = (Vint n)↑⌝ )) ∨ (callable ∗ emp)
+    )%I.
+
+  Theorem sim: HModPair.sim (InitA.Init GlobalStb) (InitI.Init) Ist.
+  Proof.
+    sim_init.
+    - (* initial condition *)
+      admit.
+    - (* init *)
+      unfold cfunU, initF, InitI.initF, interp_sb_hp, HoareFun, ccallU. s.
+      admit.
+    - (* incr *)
+      unfold cfunU, incrF, InitI.incrF, interp_sb_hp, HoareFun, ccallU. s.
+      admit.
+    - (* final *)
+      unfold cfunU, finalF, InitI.finalF, interp_sb_hp, HoareFun, ccallU. s.
+      admit.
+  Admitted.
+
+End SIM.
+
+
+
+
+(*******************************************************)
+
+
+
+
+
+
+
+
+
+
+
+
+
+
+
+
+
+
+
+
+
+
+
+
+
+
+
+
+
+
+
+
+
+
+
+
+
+
+
+
+
+
+
+
+
+
+
+
+
+
+  (* Theorem sim: HModPair.sim (InitA.Init GlobalStb) (InitI.Init) Ist.
+  Proof.
+    sim_init.
+    - (* initial condition *)
+      iIntros "H". iSplitR; eauto. steps. iRight. eauto.
+    - (* init *)
+      unfold cfunU, initF, InitI.initF, interp_sb_hp, HoareFun, ccallU. s.
+      steps. iDestruct "ASM" as "(W & (P & %))".
+      iDestruct "IST" as "[IST|IST]".
+      { iDestruct "IST" as "(P' & _)". iExFalso. iApply (pending_unique with "P P'"). }
+      iDestruct "IST" as "[C _]". subst.
+      rewrite G. steps.
+      rewrite G0. steps.
+      force. force.
+      iSplitL "C W". { iFrame. eauto. }
+      steps. iSplitL; eauto.
+      iLeft. iFrame. iPureIntro. exists (1:Z). eauto.
+    - (* incr *)
+      unfold cfunU, incrF, InitI.incrF, interp_sb_hp, HoareFun, ccallU. s.
+      steps. iDestruct "ASM" as "(W & (C & %))". subst.
+      iDestruct "IST" as "[IST|IST]"; cycle 1.
+      { iDestruct "IST" as "[C' _]". iExFalso. iApply (callable_unique with "C C'"). }
+      iDestruct "IST" as "[P N]". iDestruct "N" as ( ? ) "%". des. subst.  
+      rewrite Any.upcast_downcast in G1. inv G1. rewrite G.
+      steps. rewrite G0. steps.
+      force. force. iSplitL "W C".
+      { iFrame. eauto. }
+      steps. iSplitL; eauto.
+      { iLeft. iFrame. iPureIntro. exists (y5 + 1)%Z. eauto. }
+    - (* final *)
+      unfold cfunU, finalF, InitI.finalF, interp_sb_hp, HoareFun, ccallU. s.
+      steps. iDestruct "ASM" as "(W & (C & %))". subst.
+      rewrite G. steps. rewrite G0. steps.
+      force. force. iSplitL "W". { iFrame. eauto. }
+      steps. iFrame. eauto. 
+  Qed. *)
